



$$V_o = V_i \frac{Z_{||}}{Z_L + Z_C + Z_{||}}; G = \frac{V_o}{V_i} \Rightarrow G = \frac{1}{\frac{Z_L}{Z_{||}} + \frac{Z_C}{Z_{||}} + 1}$$

$$\Rightarrow G = \frac{1/Z_C}{\frac{1}{Z_C} + \frac{1}{Z_{||}} \left(1 + \frac{Z_L}{Z_C}\right)} = \frac{j\omega C}{j\omega C + \left(\frac{1}{R} + \frac{1}{j\omega L_m}\right) (1 + j\omega L \omega C)}$$

$$G = \frac{j\omega j\omega L_m \omega}{j\omega j\omega L_m \omega + \left(\frac{j\omega L_m \omega}{R} + 1\right) (1 + j\omega L \omega C)}$$

$$G = \frac{-\frac{L_m}{L} L C \omega^2}{\left(1 - L C \omega^2 - \frac{L_m}{L} L C \omega^2\right) + j \frac{L_m \omega}{R} (1 - L C \omega^2)}$$

$$\boxed{L_n := \frac{L_m}{L}; \quad \omega_0 = \frac{1}{\sqrt{LC}} \quad ; \quad \beta_n = \frac{\omega}{\omega_0}}$$

$$\Rightarrow \frac{L_m}{L} L C \omega^2 = L_n \left(\frac{\omega}{\omega_0}\right)^2 = L_n \beta_n^2$$

$$\begin{aligned} \text{and } L_m \frac{\omega}{R} &= \frac{L_m}{L} \sqrt{L} \sqrt{L} \frac{\omega}{R} = L_n \sqrt{\frac{L}{C}} \cdot \frac{1}{R} \omega \sqrt{LC} \\ &= L_n \frac{\omega}{\omega_0} \frac{\sqrt{L/C}}{R} \\ &= L_n \beta_n \mathcal{P} \quad \text{where } \boxed{\mathcal{P} =: \frac{\sqrt{L/C}}{R}} \end{aligned}$$

$$\text{So: } G = \frac{L_n \beta_n^2}{(\beta_n^2 + L_n \beta_n^2 - 1) + j L_n \mathcal{P} \beta_n (-1 + \beta_n^2)}$$

$$\boxed{G = \frac{L_n \beta_n^2}{[\beta_n^2 (1 + L_n) - 1] + j L_n \mathcal{P} \beta_n [\beta_n^2 - 1]}}$$